example.v
@@ -1,3 +1,14 @@
+(*
+  A nice example of λ-Pallene code:
+
+  let A:tbl[tbl[int]] = {} : tbl[tbl[int]] in
+  let B:tbl[int] = (A as tbl[int]) in
+    A[1] = B; B[2] = 10; A[1][2]
+
+  It types and reduces to 10.
+*)
+
+
 Require Import Coq.Logic.Decidable.
 Require Import PeanoNat.
 Require Import Coq.Strings.String.
@@ -10,78 +21,58 @@ Require Import LIR.maps.
 Require Import LIR.pallene.
 Require Import LIR.lir.
 
-(*
-  A nice example of λ-Pallene code:
-
-  let A:tbl[tbl[int]] = {} : tbl[tbl[int]] in
-  let B:tbl[int] = (A as tbl[int]) in
-    A[1] = B; B[2] = 10; A[1][2]
-*)
-
+(* Sequence 'operator' e1 ; e2 *)
+Definition PESeq (e1 e2 : PE) : PE := PELet ("":string) PTNil e1 e2.
 
 Definition example :=
     PELet ("A":string) (PTArr (PTArr PTInt)) (PENew (PTArr PTInt))
     (PELet ("B":string) (PTArr PTInt)
                         (PECast (PEVar ("A":string)) (PTArr PTInt))
-     (PELet ("":string) PTNil
+     (PESeq
        (PESet (PEVar ("A":string)) (PENum 1) (PEVar ("B":string)))
-    (PELet ("":string) PTNil
+      (PESeq
        (PESet (PEVar ("B":string)) (PENum 2) (PENum 10))
        (PEGet (PEGet (PEVar ("A":string)) (PENum 1)) (PENum 2))))).
-       
 
-(* Example is well typed with type int *)
+
+(*
+** Example is well typed with type int
+*)
 Goal typeOf MEmpty example = Some PTInt.
 Proof. trivial. Qed.
 
 
 (*
-** Multistep
+** Example evaluates to 10
 *)
-Reserved Notation "m '/' e '-p->*' m1 '/' e1"
-(at level 40, e at level 39, m1 at level 39, e1 at level 39).
-Reserved Notation "m '/' e '-p->*' 'fail'"
-(at level 40, e at level 39).
-
-Inductive multistep : PMem -> PE -> PMem -> PE -> Prop :=
-| MStRefl : forall m e, m / e -p->* m / e
-| MStMStep : forall m e m' e' m'' e'',
-    m / e -p-> m' / e' ->
-    m' / e' -p->* m'' / e'' ->
-    m / e -p->* m'' / e''
-
-where "m / e -p->* m1 / e1" := (multistep m e m1 e1)
-.
-
-(* example evaluates to 10 *)
 Lemma run : exists m, PEmptyMem / example -p->* m / (PENum 10).
 Proof with eauto 10 using pstep, PValue.
   eexists.
   unfold example.
-  eapply MStMStep.
+  eapply PMStMStep.
   { eapply PStLet1. eapply PStNew. unfold PfreshT. simpl. eauto. }
-  eapply MStMStep...  (* Let *)
-  eapply MStMStep.
+  eapply PMStMStep...  (* Let *)
+  eapply PMStMStep.
   { eapply PStLet1. simpl. eapply PStCast; eauto using PValue.
     discriminate. simpl. trivial. }
   simpl.
-  eapply MStMStep...  (* Let *)
-  eapply MStMStep.
+  eapply PMStMStep...  (* Let *)
+  eapply PMStMStep.
   { eapply PStLet1. simpl. eapply PStSet. auto using PValue. }
   simpl.
-  eapply MStMStep...  (* Let *)
-  eapply MStMStep.
+  eapply PMStMStep...  (* Let *)
+  eapply PMStMStep.
   { eapply PStLet1. eapply PStSet. auto using PValue. }
-  eapply MStMStep...  (* Let *)
-  eapply MStMStep...  (* Get *)
+  eapply PMStMStep...  (* Let *)
+  eapply PMStMStep...  (* Get *)
   simpl.
-  eapply MStMStep.
+  eapply PMStMStep.
   { eapply PStGet1. eapply PStCast; auto using PValue; easy. }
-  eapply MStMStep...  (* Get *)
+  eapply PMStMStep...  (* Get *)
   simpl.
-  eapply MStMStep.
+  eapply PMStMStep.
   { eapply PStCast; auto using PValue; easy. }
-  eauto using multistep.
+  eauto using Pmultistep.
   Unshelve. all: auto using PValue.
 Qed.
 
